
The GFCTP-E formulation is as follows:

%%% 
\begin{subequations}\label{eqs:GFCTP-E}
  \begin{align}
    %%
    \min_{z} \:\: & 
    z = \sum_{h \in H}\sum_{i \in I}\sum_{j \in J}c_{i,j}(h) x_{i,j}(h) 
    & \label{eq:GRCTP-E_obj} \\
    %%
    \text{s.t.} \:\: &
    \sum_{j \in J}\beta_{i,k}(h,q_{j}) x_{i,j}(h) \leq S_{i,k}(h) 
    & 
    \forall \: i \in I, \: \forall \: k \in K_{i}(h) \label{eq:GRCTP-E_sup} \\
    %%
    &
    \sum_{i \in I}\sum_{h \in H_{j}} x_{i,j}(h) \geq d_{j}(H_{j}) 
    & 
    \forall \: j \in J_{o} \label{eq:GRCTP-E_dem} \\
    %%
    &
    \sum_{i \in I}\sum_{h \in H_{j}} y_{i,j} x_{i,j}(h) \geq d_{j}(H_{j}) 
    &
    \forall \: j \in J_{e} \label{eq:GRCTP-E_dem_e} \\
    %%
    &
    \sum_{i \in I} y_{i,j} = 1
    &
    \forall \: j \in J_{e} \label{eq:GRCTP-E_sumy} \\
    %%
    &
    x_{i,j} \geq 0
    &
    \forall \: x \in X \label{eq:GRCTP-E_x} \\
    %%
    &
    y_{i,j} \in \{0,1\}
    &
    \forall \: y \in Y \label{eq:GRCTP-E_y}
    %%
  \end{align}
\end{subequations}
%%% 
